CertiGC/verif_forward.v
@@ -38,85 +38,89 @@ Qed.
 Lemma body_forward: semax_body Vprog Gprog f_forward forward_spec.
 Proof.
   start_function.
-  rename H3 into HC. rename H4 into HT. unfold forward_p_address. destruct forward_p.
-  - unfold thread_info_rep. Intros. hnf in H0. destruct H as [? [? [? ?]]]. hnf in H3.
+  destruct H as [? [? [? ?]]]. destruct H1 as [? [? [? ?]]]. unfold forward_p_address.
+  destruct forward_p.
+  - unfold thread_info_rep. Intros.
     assert (Zlength roots = Zlength (live_roots_indices f_info)). {
       rewrite <- (Zlength_map _ _ (flip Znth (ti_args t_info))), <- H3, Zlength_map.
       reflexivity. }
-    pose proof (Znth_map _ (root2val g) _ H0). rewrite H6 in H0.
-    rewrite H3, Znth_map in H7 by assumption. unfold flip in H7.
-    remember (Znth z roots) as root. rewrite <- H6 in H0. pose proof (Znth_In _ _ H0).
-    rewrite <- Heqroot in H8. rewrite H6 in H0. unfold Inhabitant_val in H7.
+    pose proof (Znth_map _ (root2val g) _ H0). hnf in H0. rewrite H9 in H0.
+    rewrite H3, Znth_map in H10 by assumption. unfold flip in H10.
+    remember (Znth z roots) as root. rewrite <- H9 in H0. pose proof (Znth_In _ _ H0).
+    rewrite <- Heqroot in H11. rewrite H9 in H0. unfold Inhabitant_val in H10.
     assert (forall v, In (inr v) roots -> isptr (vertex_address g v)). {
-      intros. destruct H4. unfold vertex_address. rewrite Forall_forall in H10.
-      rewrite (filter_sum_right_In_iff v roots) in H9. apply H10 in H9. destruct H9.
-      apply graph_has_gen_start_isptr in H9.
+      intros. destruct H4. unfold vertex_address. rewrite Forall_forall in H13.
+      rewrite (filter_sum_right_In_iff v roots) in H12. apply H13 in H12.
+      destruct H12. apply graph_has_gen_start_isptr in H12.
       remember (gen_start g (vgeneration v)) as vv. destruct vv; try contradiction.
       simpl. exact I. }
     assert (is_pointer_or_integer (root2val g root)). {
       destruct root as [[? | ?] | ?]; simpl; auto.
       - destruct g0. simpl. exact I.
-      - specialize (H9 _ H8). apply isptr_is_pointer_or_integer. assumption. }
-    assert (HB: 0 <= Znth z (live_roots_indices f_info) < 1024) by
+      - specialize (H12 _ H11). apply isptr_is_pointer_or_integer. assumption. }
+    assert (0 <= Znth z (live_roots_indices f_info) < 1024) by
         (apply (fi_index_range f_info), Znth_In; assumption).
-    forward; rewrite H7. 1: entailer!.
+    forward; rewrite H10. 1: entailer!.
     assert_PROP (valid_int_or_ptr (root2val g root)). {
-      gather_SEP 3 2. sep_apply (root_valid_int_or_ptr _ _ _ _ H8 H4). entailer!. }
+      gather_SEP 3 2. sep_apply (root_valid_int_or_ptr _ _ _ _ H11 H4). entailer!. }
     forward_call (root2val g root).
     remember (graph_rep g * heap_rest_rep (ti_heap t_info) * outlier_rep outlier)
-      as P. pose proof (graph_and_heap_rest_data_at_ _ _ _ H1 H).
-    unfold generation_data_at_ in H12. remember (gen_start g from) as fp.
+      as P. pose proof (graph_and_heap_rest_data_at_ _ _ _ H6 H).
+    unfold generation_data_at_ in H16. remember (gen_start g from) as fp.
     remember (nth_sh g from) as fsh. remember (gen_size t_info from) as gn.
     remember (WORD_SIZE * gn)%Z as fn.
     assert (P |-- (weak_derives P (memory_block fsh fn fp * TT) && emp) * P). {
-      apply weak_derives_strong. subst. sep_apply H12.
+      apply weak_derives_strong. subst. sep_apply H16.
       rewrite data_at__memory_block.
       rewrite sizeof_tarray_int_or_ptr; [Intros; cancel | unfold gen_size].
       destruct (total_space_tight_range (nth_space t_info from)). assumption. }
     destruct root as [[? | ?] | ?]; simpl root2val.
     + unfold odd_Z2val. apply semax_if_seq. forward_if.
-      1: exfalso; apply H14'; reflexivity.
+      1: exfalso; apply H18'; reflexivity.
       forward. Exists g t_info roots. rewrite <- Heqroot. entailer!.
-      * simpl. constructor.
+      * simpl. split; [constructor | hnf; intuition].
       * unfold thread_info_rep. entailer!.
     + unfold GC_Pointer2val. destruct g0. apply semax_if_seq. forward_if.
-      2: exfalso; apply Int.one_not_zero in H14; assumption.
+      2: exfalso; apply Int.one_not_zero in H18; assumption.
       forward_call (Vptr b i). gather_SEP 3 6 2. rewrite <- sepcon_assoc.
       rewrite <- HeqP. destruct H4.
       replace_SEP 0 ((weak_derives P (memory_block fsh fn fp * TT) && emp) * P) by
-          (entailer; assumption). clear H13. Intros. simpl root2val in *.
+          (entailer; assumption). clear H17. Intros. simpl root2val in *.
       assert (P |-- (weak_derives P (valid_pointer (Vptr b i) * TT) && emp) * P). {
         subst. cancel. apply andp_right. 2: cancel.
         assert (HS: emp |-- TT) by entailer; sep_apply HS; clear HS.
         apply derives_weak.
-        sep_apply (outlier_rep_valid_pointer roots outlier (GCPtr b i) H8 H4).
+        sep_apply (outlier_rep_valid_pointer roots outlier (GCPtr b i) H11 H4).
         simpl GC_Pointer2val. cancel. }
       replace_SEP 1 ((weak_derives P (valid_pointer (Vptr b i) * TT) && emp) * P) by
-          (entailer; assumption). Intros. clear H13.
+          (entailer; assumption). Intros. clear H17.
       forward_call (fsh, fp, fn, (Vptr b i), P). Intros v. destruct v.
-      * rewrite HeqP. Intros. gather_SEP 0 1. sep_apply H12. rewrite Heqfn in v.
-        sep_apply (outlier_rep_single_rep _ _ _ H8 H4). Intros. gather_SEP 0 2.
+      * rewrite HeqP. Intros. gather_SEP 0 1. sep_apply H16. rewrite Heqfn in v.
+        sep_apply (outlier_rep_single_rep _ _ _ H11 H4). Intros. gather_SEP 0 2.
         change (Vptr b i) with (GC_Pointer2val (GCPtr b i)) in v.
         pose proof (generation_share_writable (nth_gen g from)).
-        change (generation_sh (nth_gen g from)) with (nth_sh g from) in H13.
-        rewrite <- Heqfsh in H13. unfold generation_data_at_.
-        sep_apply (single_outlier_rep_memory_block_FF (GCPtr b i) fp gn fsh H13 v).
+        change (generation_sh (nth_gen g from)) with (nth_sh g from) in H17.
+        rewrite <- Heqfsh in H17. unfold generation_data_at_.
+        sep_apply (single_outlier_rep_memory_block_FF (GCPtr b i) fp gn fsh H17 v).
         assert_PROP False by entailer!. contradiction.
-      * apply semax_if_seq. forward_if. 1: exfalso; apply H13'; reflexivity.
+      * apply semax_if_seq. forward_if. 1: exfalso; apply H17'; reflexivity.
         forward. Exists g t_info roots. rewrite <- Heqroot. entailer!.
-        -- unfold roots_compatible. intuition. simpl. constructor.
+        -- split; [|split].
+           ++ unfold roots_compatible. split; assumption.
+           ++ simpl; constructor.
+           ++ hnf; intuition.
         -- unfold thread_info_rep. entailer!.
-    + specialize (H9 _ H8). destruct (vertex_address g v) eqn:? ; try contradiction.
+    + specialize (H12 _ H11). destruct (vertex_address g v) eqn:? ; try contradiction.
       apply semax_if_seq. forward_if.
-      2: exfalso; apply Int.one_not_zero in H14; assumption.
-      clear H14 H14'. simpl in H11, H10. forward_call (Vptr b i).
+      2: exfalso; apply Int.one_not_zero in H18; assumption.
+      clear H18 H18'. simpl in H13, H15. forward_call (Vptr b i).
       rewrite <- Heqv0 in *. gather_SEP 3 6 2. rewrite <- sepcon_assoc, <- HeqP.
       replace_SEP 0 ((weak_derives P (memory_block fsh fn fp * TT) && emp) * P) by
-          (entailer; assumption). clear H13. Intros. assert (graph_has_v g v). {
-        destruct H4. rewrite Forall_forall in H13. apply H13.
+          (entailer; assumption). clear H17. Intros. assert (graph_has_v g v). {
+        destruct H4. rewrite Forall_forall in H17. apply H17.
         rewrite <- filter_sum_right_In_iff. assumption. }
       assert (P |-- (weak_derives P (valid_pointer (Vptr b i) * TT) && emp) * P). {
-        apply weak_derives_strong. subst. sep_apply (graph_rep_vertex_rep g v H13).
+        apply weak_derives_strong. subst. sep_apply (graph_rep_vertex_rep g v H17).
         Intros shh. unfold vertex_rep, vertex_at. remember (make_fields_vals g v).
         sep_apply (data_at_valid_ptr shh (tarray int_or_ptr_type (Zlength l)) l
                                      (vertex_address g v)).
@@ -125,14 +129,13 @@ Proof.
           rewrite Z.max_r; pose proof (raw_fields_range (vlabel g v)); omega.
         - rewrite Heqv0; cancel. }
       replace_SEP 1 (weak_derives P (valid_pointer (Vptr b i) * TT) && emp * P)
-        by (entailer; assumption). clear H14. Intros. rewrite <- Heqv0 in *.
+        by (entailer; assumption). clear H18. Intros. rewrite <- Heqv0 in *.
       forward_call (fsh, fp, fn, (vertex_address g v), P). Intros vv. rewrite HeqP.
-      sep_apply (graph_and_heap_rest_v_in_range_iff _ _ _ _ H H1 H13). Intros.
-      rewrite <- Heqfp, <- Heqgn, <- Heqfn in H14. destruct vv.
-      * Intros. rewrite H14 in v0. clear H14. apply semax_if_seq. forward_if.
-        2: exfalso; inversion H14. deadvars!. freeze [1; 2; 3; 4; 5; 6] FR.
-        clear H14 H14'.
-        localize [vertex_rep (nth_sh g (vgeneration v)) g v].
+      sep_apply (graph_and_heap_rest_v_in_range_iff _ _ _ _ H H6 H17). Intros.
+      rewrite <- Heqfp, <- Heqgn, <- Heqfn in H18. destruct vv.
+      * Intros. rewrite H18 in v0. clear H18. apply semax_if_seq. forward_if.
+        2: exfalso; inversion H18. deadvars!. freeze [1; 2; 3; 4; 5; 6] FR.
+        clear H18 H18'. localize [vertex_rep (nth_sh g (vgeneration v)) g v].
         unfold vertex_rep, vertex_at. Intros. rewrite v0.
         assert (readable_share (nth_sh g from)) by
             (unfold nth_sh; apply writable_readable, generation_share_writable).
@@ -146,11 +149,11 @@ Proof.
           reflexivity. } forward.
         gather_SEP 0 1. replace_SEP 0 (vertex_rep (nth_sh g (vgeneration v)) g v) by
             (unfold vertex_rep, vertex_at; entailer!).
-        unlocalize [graph_rep g]. 1: apply (graph_vertex_ramif_stable _ _ H13).
-        apply semax_if_seq. forward_if; rewrite make_header_int_rep_mark_iff in H16.
+        unlocalize [graph_rep g]. 1: apply (graph_vertex_ramif_stable _ _ H17).
+        apply semax_if_seq. forward_if; rewrite make_header_int_rep_mark_iff in H20.
         -- deadvars!. localize [vertex_rep (nth_sh g (vgeneration v)) g v].
            rewrite v0. unfold vertex_rep, vertex_at. Intros.
-           unfold make_fields_vals at 2. rewrite H16.
+           unfold make_fields_vals at 2. rewrite H20.
            assert (0 <= 0 < Zlength (make_fields_vals g v)). {
              split. 1: omega. rewrite fields_eq_length.
              apply (proj1 (raw_fields_range (vlabel g v))). }
@@ -158,34 +161,35 @@ Proof.
                      (vertex_address g (copied_vertex (vlabel g v)))). {
              apply isptr_is_pointer_or_integer. unfold vertex_address.
              rewrite isptr_offset_val.
-             apply graph_has_gen_start_isptr, HC; assumption. }
+             apply graph_has_gen_start_isptr, H8; assumption. }
            forward. rewrite Znth_0_cons. gather_SEP 0 1.
            replace_SEP 0 (vertex_rep (nth_sh g (vgeneration v)) g v). {
              unfold vertex_rep, vertex_at. unfold make_fields_vals at 3.
-             rewrite H16. entailer!. }
-           unlocalize [graph_rep g]. 1: apply (graph_vertex_ramif_stable _ _ H13).
+             rewrite H20. entailer!. }
+           unlocalize [graph_rep g]. 1: apply (graph_vertex_ramif_stable _ _ H17).
            thaw FR. forward. forward. rewrite <- Heqroot.
-           rewrite if_true by reflexivity. rewrite H16.
+           rewrite if_true by reflexivity. rewrite H20.
            Exists g (upd_thread_info_arg
                        t_info
                        (Znth z (live_roots_indices f_info))
-                       (vertex_address g (copied_vertex (vlabel g v))) HB)
+                       (vertex_address g (copied_vertex (vlabel g v))) H14)
                   (upd_bunch z f_info roots (inr (copied_vertex (vlabel g v)))).
-           unfold thread_info_rep. simpl. entailer!. split; [split|].
+           unfold thread_info_rep. simpl. entailer!. split; split.
            ++ apply upd_fun_thread_arg_compatible. assumption.
-           ++ specialize (HC _ H13 H16). apply upd_roots_compatible; assumption.
+           ++ specialize (H8 _ H17 H20). apply upd_roots_compatible; assumption.
            ++ apply fr_v_in_forwarded; [reflexivity | assumption].
+           ++ hnf. intuition.
         -- forward. deadvars!. thaw FR. freeze [0; 1; 2; 3; 4; 5] FR.
            rewrite make_header_Wosize by (apply not_true_is_false; assumption).
            assert (0 <= Z.of_nat to < 12). {
-             clear -H H2. destruct H as [_ [_ ?]]. red in H2.
+             clear -H H7. destruct H as [_ [_ ?]]. red in H7.
              pose proof (spaces_size (ti_heap t_info)).
              rewrite Zlength_correct in H0. rep_omega. }
            assert (0 < Z.of_nat to) by omega. unfold heap_struct_rep.
            remember (Znth (Z.of_nat to) (spaces (ti_heap t_info))) as sp_to.
            assert (isptr (space_start sp_to)). {
-             destruct (gt_gs_compatible _ _ H _ H2) as [? _]. subst sp_to.
-             rewrite nth_space_Znth in H19. rewrite <- H19. apply start_isptr. }
+             destruct (gt_gs_compatible _ _ H _ H7) as [? _]. subst sp_to.
+             rewrite nth_space_Znth in H23. rewrite <- H23. apply start_isptr. }
            remember ((space_start (heap_head (ti_heap t_info)),
                       (Vundef,
                        offset_val
@@ -197,17 +201,17 @@ Proof.
              rewrite map_tl, Znth_tl by omega.
              replace (Z.of_nat to - 1 + 1) with (Z.of_nat to) by omega.
              rewrite Znth_map by (rewrite spaces_size; rep_omega). reflexivity. }
-           unfold Inhabitant_pair, Inhabitant_val, Inhabitant in H20.
-           forward; rewrite H20; unfold space_tri. 1: entailer!.
+           unfold Inhabitant_pair, Inhabitant_val, Inhabitant in H24.
+           forward; rewrite H24; unfold space_tri. 1: entailer!.
            forward. simpl sem_binary_operation'.
            rewrite sapi_ptr_val by assumption. Opaque Znth. forward. Transparent Znth.
-           rewrite sapi_ptr_val by assumption. rewrite H20. unfold space_tri.
+           rewrite sapi_ptr_val by assumption. rewrite H24. unfold space_tri.
            rewrite <- Z.add_assoc.
            replace (1 + Zlength (raw_fields (vlabel g v))) with (vertex_size g v) by
                (unfold vertex_size; omega). admit.
-      * apply semax_if_seq. forward_if. 1: exfalso; apply H15'; reflexivity.
-        rewrite H14 in n. forward. rewrite <- Heqroot. rewrite if_false by assumption.
+      * apply semax_if_seq. forward_if. 1: exfalso; apply H19'; reflexivity.
+        rewrite H18 in n. forward. rewrite <- Heqroot. rewrite if_false by assumption.
         Exists g t_info roots. simpl. entailer!.
-        -- constructor. assumption.
+        -- split; [constructor; assumption | hnf; intuition].
         -- unfold thread_info_rep. entailer!.
 Abort.
